proof semantic eq (on direction)

src/parlang_nonmono.lean
@@ -44,7 +44,56 @@ def contains_sync : kernel σ τ → Prop
 
 instance decidable (k : kernel σ τ) : decidable (contains_sync k) := sorry
 
-variables {s t : state n σ τ} {ac : vector bool n}
+variables {s t u : state n σ τ} {ac : vector bool n} {f f' : σ → bool} {semantics : kernel σ τ → vector bool n → state n σ τ → state n σ τ → Prop}
+
+class has_unique (semantics : kernel σ τ → vector bool n → state n σ τ → state n σ τ → Prop) := 
+(unique : ∀ {k : kernel σ τ} {ac : vector bool n} {s t t' : state n σ τ}, semantics k ac s t → semantics k ac s t' → t = t')
+
+variables [has_unique semantics]
+
+instance unique2 : has_unique $ @parlang.exec_state σ ι τ _ n := ⟨begin
+    intros _ _ _ _ _ a b,
+    apply parlang.exec_state_unique b a,
+end⟩
+
+instance unique1 : has_unique $ @exec_state σ ι τ _ n := sorry
+
+def ac_ge (ac' : vector bool n) (ac : vector bool n) : Prop := ∀ (t : fin n), ¬ (ac.nth t) → ¬ (ac'.nth t)
+
+instance : has_le (vector bool n) := ⟨ac_ge⟩
+
+lemma exec_state_inactive_threads_untouched {s u : state n σ τ} {ac : vector bool n} {k} : exec_state k ac s u → ∀ i, ¬ ac.nth i → s.threads.nth i = u.threads.nth i := begin
+    admit,
+end
+
+lemma monotonic_exec {f k} : 
+exec_state k (deactivate_threads (bnot ∘ f) ac s) s t →
+deactivate_threads (bnot ∘ f) ac s ≥ deactivate_threads (bnot ∘ f) ac t := begin
+    intro h,
+    intros tid,
+    unfold deactivate_threads,
+    repeat { rw vector.nth_map },
+    repeat { rw vector.nth_map₂ },
+    repeat { rw deactivate_threads._match_1 },
+    repeat { rw band_coe_iff },
+    intros hna ha,
+    cases ha,
+    apply hna,
+    clear hna,
+    split, 
+    {
+        simp only [bool.bnot_bnot] at ha_left,
+        simp only [bool.bnot_bnot],
+        by_cases e : f ((vector.nth (s.threads) tid).tlocal) = tt,
+        { assumption, },
+        rw exec_state_inactive_threads_untouched h tid,
+        assumption,
+        simp [deactivate_threads, *],
+        sorry, -- trivial
+    }, {
+        assumption,
+    }
+end
 
 -- probably has to be an inducive type
 -- def ac_after_n_iteration (k : kernel σ τ) (f : σ → bool) : ℕ → state n σ τ → vector bool n → vector bool n
@@ -53,19 +102,56 @@ variables {s t : state n σ τ} {ac : vector bool n}
 
 -- this is similar to the semantic itself except we are not interested in states but the resulting active maps
 -- it is reversed, maybe we should build it the other way around
-inductive ac_after_n_iteration (semantics : Π {σ ι : Type} {τ : ι → Type} [_inst_1 : decidable_eq ι] {n : ℕ}, kernel σ τ → vector bool n → state n σ τ → state n σ τ → Prop) (k : kernel σ τ) (f : σ → bool) : state n σ τ → vector bool n → vector bool n → ℕ → Prop
+inductive ac_after_n_iteration (semantics : kernel σ τ → vector bool n → state n σ τ → state n σ τ → Prop) (k : kernel σ τ) (f : σ → bool) : state n σ τ → vector bool n → vector bool n → ℕ → Prop
 | base (ac : vector bool n) (s : state n σ τ) : ac_after_n_iteration s ac ac 0
-| step (ac : vector bool n) (s t : state n σ τ) (i : ℕ) (ac' : vector bool n) : ac_after_n_iteration t (deactivate_threads (bnot ∘ f) ac t) ac' i → semantics k ac s t → ac_after_n_iteration s ac ac' (i + 1)
+| step {ac : vector bool n} (s t : state n σ τ) {i : ℕ} {ac' : vector bool n} : ac_after_n_iteration t (deactivate_threads (bnot ∘ f) ac s) ac' i → semantics k (deactivate_threads (bnot ∘ f) ac s) s t → ac_after_n_iteration s ac ac' (i + 1)
 --| step (ac : vector bool n) (s t : state n σ τ) (i : ℕ) (ac' : vector bool n) : ac_after_n_iteration s ac ac' i → exec_state k ac' s t → ac_after_n_iteration s ac (deactivate_threads (bnot ∘ f) ac t) (i + 1)
 
-lemma ac_after_n_iteration_unique {k : kernel σ τ} {f : σ → bool} {ac' ac'' : vector bool n} {i} : 
-ac_after_n_iteration @parlang.exec_state k f s ac ac' i → ac_after_n_iteration @parlang.exec_state k f s ac ac'' i → ac' = ac'' := begin
-    admit,
+-- this semantic would require that in and out ac are always the same
+inductive ac_after_n_iteration_nonmono (semantics : kernel σ τ → vector bool n → state n σ τ → state n σ τ → Prop) (k : kernel σ τ) (f : σ → bool) : state n σ τ → vector bool n → vector bool n → ℕ → Prop
+| base (ac : vector bool n) (s : state n σ τ) : ac_after_n_iteration_nonmono s ac ac 0
+| step {ac : vector bool n} (s t : state n σ τ) {i : ℕ} {ac' : vector bool n} : ac_after_n_iteration_nonmono t ac ac' i → semantics k (deactivate_threads (bnot ∘ f) ac s) s t → ac_after_n_iteration_nonmono s ac ac' (i + 1)
+
+example {k f} {ac' : vector bool n} {i} : ac_after_n_iteration semantics k f s ac ac' i ↔ ac_after_n_iteration_nonmono semantics k f s ac ac' i := begin
+    split, {
+        revert ac ac' s,
+        induction i,
+        case nat.zero {
+            intros ac ac' s h,
+            cases h,
+            apply ac_after_n_iteration_nonmono.base,
+        },
+        case nat.succ {
+            intros ac ac' s h,
+            cases h,
+            rename h_t t,
+            apply ac_after_n_iteration_nonmono.step,
+            swap,
+            exact h_a_1,
+            apply i_ih,
+            clear i_ih,
+            cases i_n,
+            case nat.zero {
+
+            }
+            
+        }
+    }
 end
 
-def ac_ge (ac' : vector bool n) (ac : vector bool n) : Prop := ∀ (t : fin n), ¬ (ac.nth t) → ¬ (ac'.nth t)
+notation `v[` v:(foldr `, ` (h t, vector.cons h t) vector.nil `]`) := v
 
-instance : has_le (vector bool n) := ⟨ac_ge⟩
+example : ac_after_n_iteration exec_state (compute (λ (m : bool), ff)) id (@parlang.init_state bool string (λs, ℕ) _ (λ_, tt) (λ_,1) (λs:string, 0)) v[tt] v[tt] 1 := begin
+    apply ac_after_n_iteration.step _ (@parlang.init_state bool string (λs, ℕ) _ (λ_, ff) (λ_,1) (λs:string, 0)),
+    swap,
+    sorry,
+    apply ac_after_n_iteration.base,
+end
+
+lemma ac_after_n_iteration_unique {k : kernel σ τ} {f : σ → bool} {ac' ac'' : vector bool n} {i} : 
+ac_after_n_iteration semantics k f s ac ac' i → ac_after_n_iteration semantics k f s ac ac'' i → ac' = ac'' := begin
+    admit,
+end
 
 lemma ac_sub_deac {f : σ → bool} : ac ≥ (deactivate_threads (bnot ∘ f) ac s) := begin
     intros t h₁ h₂,
@@ -79,7 +165,25 @@ lemma ac_sub_deac {f : σ → bool} : ac ≥ (deactivate_threads (bnot ∘ f) ac
     assumption,
 end
 
-lemma ac_ge_single {k : kernel σ τ} {f : σ → bool} {ac' : vector bool n} {i : ℕ} : ac_after_n_iteration @parlang.exec_state k f s ac ac' i → ac ≥ ac' := begin
+lemma ac_deac_comm : deactivate_threads f (deactivate_threads f' ac s) t = deactivate_threads f' (deactivate_threads f ac t) s := begin
+    induction n,
+    case nat.zero {
+        apply vector.vector_0_eq',
+    },
+    case nat.succ {
+        sorry,
+    }
+end
+
+lemma ac_trans {ac' ac'' : vector bool n} : ac ≥ ac' → ac' ≥ ac'' → ac ≥ ac'' := begin
+    admit,
+end
+
+lemma ac_deac_ge (h : deactivate_threads f ac s ≥ deactivate_threads f' ac t) : deactivate_threads f' (deactivate_threads f ac s) t = deactivate_threads f' ac t := begin
+    admit,
+end
+
+lemma ac_ge_single {k : kernel σ τ} {f : σ → bool} {ac' : vector bool n} {i : ℕ} : ac_after_n_iteration semantics k f s ac ac' i → ac ≥ ac' := begin
     intros h,
     induction i generalizing s ac ac',
     case nat.zero {
@@ -95,27 +199,8 @@ lemma ac_ge_single {k : kernel σ τ} {f : σ → bool} {ac' : vector bool n} {i
     }
 end
 
-example {ac' ac'' : vector bool n} {k : kernel σ τ} {f : σ → bool} {i : ℕ} : 
-ac_after_n_iteration @parlang.exec_state k f s ac ac' i → ac_after_n_iteration @parlang.exec_state k f s ac ac'' (i + 1) → ac' ≥ ac'' := begin
-    intros h₁ h₂,
-    induction i generalizing s ac,
-    case nat.zero {
-        cases h₁,
-        cases h₂,
-        cases h₂_a,
-        apply ac_sub_deac,
-    },
-    case nat.succ {
-        cases h₁,
-        cases h₂,
-        have : h₁_t = h₂_t := exec_state_unique h₂_a_1 h₁_a_1,
-        subst this,
-        apply i_ih h₁_a h₂_a,
-    }
-end
-
 lemma ac_ge_two {k : kernel σ τ} {f : σ → bool} {i i' : ℕ} {ac' ac'' : vector bool n} : 
-ac_after_n_iteration @parlang.exec_state k f s ac ac' i → ac_after_n_iteration @parlang.exec_state k f s ac ac'' (i + i') → ac' ≥ ac'' := begin
+ac_after_n_iteration semantics k f s ac ac' i → ac_after_n_iteration semantics k f s ac ac'' (i + i') → ac' ≥ ac'' := begin
     intros h₁ h₂,
     induction i generalizing s ac,
     case nat.zero {
@@ -127,14 +212,135 @@ ac_after_n_iteration @parlang.exec_state k f s ac ac' i → ac_after_n_iteration
         have : nat.succ i_n + i' = nat.succ (i_n + i') := by rw nat.succ_add,
         rw this at h₂,
         cases h₂,
-        have : h₁_t = h₂_t := exec_state_unique h₂_a_1 h₁_a_1,
+        have : h₁_t = h₂_t := has_unique.unique _ _ _ h₁_a_1 h₂_a_1,
         subst this,
         apply i_ih h₁_a h₂_a,
     }
 end
 
-def monotone_loop (f k) (s : state n σ τ) (ac : vector bool n) : Prop := 
-∀ (i i' : ℕ) (ac' ac'' : vector bool n), ac_after_n_iteration @parlang.exec_state k f s ac ac' i → ac_after_n_iteration @parlang.exec_state k f s ac ac'' (i + i') → ac' ≥ ac''
+#print parlang_nonmono.exec_state.rec_on
+
+lemma loop_ac {k : kernel σ τ}  (h : exec_state (loop f k) ac s t) : ∃ i ac', ac_after_n_iteration exec_state k f s ac ac' i ∧ no_thread_active (deactivate_threads (bnot ∘ f) ac' t)
+:= h.rec_on 
+    (λ f s ac, _)
+    _
+    _
+    _
+    _
+    _
+    _
+    _
+    (λ s t u ac f k h₁ h₂ h₃ ih₁ (ih₂ : ∃ (i : ℕ) (ac' : vector bool n), ac_after_n_iteration exec_state k f s ac ac' i ∧ ↥(no_thread_active (deactivate_threads (bnot ∘ f) ac' t))), (show ∃ i ac', ac_after_n_iteration exec_state k f s ac ac' i ∧ no_thread_active (deactivate_threads (bnot ∘ f) ac' t), by begin 
+
+    end))
+
+def monotone_loop (semantics : kernel σ τ → vector bool n → state n σ τ → state n σ τ → Prop) (f k) (s : state n σ τ) (ac : vector bool n) : Prop := 
+∀ (i i' : ℕ) (ac' ac'' : vector bool n), ac_after_n_iteration semantics k f s ac ac' i → ac_after_n_iteration semantics k f s ac ac'' (i + i') → ac' ≥ ac''
+
+lemma par_loop_ac' {k : kernel σ τ} : parlang.exec_state (loop f k) ac s t → ∃ i ac', ac_after_n_iteration parlang.exec_state k f s ac ac' i ∧ no_thread_active (deactivate_threads (bnot ∘ f) ac' t) := begin
+    generalize eq_l : (loop f k) = l,
+    intro h,
+    induction h;
+        cases eq_l,
+    {
+        use 0,
+        use h_ac,
+        split,
+        apply ac_after_n_iteration.base,
+        assumption,
+    }, {
+        clear h_ih_a,
+        specialize h_ih_a_1 rfl,
+        cases h_ih_a_1 with i ih,
+        cases ih with ac' ih,
+        cases ih with ha hb,
+        use i + 1,
+        use ac',
+        split,
+        swap,
+        assumption,
+        apply ac_after_n_iteration.step,
+        repeat { assumption },
+    }
+end
+
+lemma loop_ac' {k : kernel σ τ} : exec_state (loop f k) ac s t ↔ ∃ i ac', ac_after_n_iteration exec_state k f s ac ac' i ∧ no_thread_active (deactivate_threads (bnot ∘ f) ac' t) := begin
+    split,
+    {
+        generalize eq_l : (loop f k) = l,
+        intro h,
+        induction h generalizing;
+            cases eq_l,
+        {
+            use 0,
+            use h_ac,
+            split,
+            apply ac_after_n_iteration.base,
+            assumption,
+        }, {
+            clear h_ih_a,
+            specialize h_ih_a_1 rfl,
+            cases h_ih_a_1 with i ih,
+            cases ih with ac' ih,
+            cases ih with ha hb,
+            use i + 1,
+            use ac',
+            split,
+            swap,
+            assumption,
+            {
+                apply ac_after_n_iteration.step,
+                swap,
+                exact h_a_1,
+                induction ha,
+                case parlang_nonmono.ac_after_n_iteration.base {
+                    have : monotone_loop exec_state f k h_s ha_ac := by apply ac_ge_two,
+                    have : monotone_loop exec_state f k h_s ha_ac := by apply ac_ge_two,
+                }
+            }
+        }
+    }
+end
+
+#print loop_ac'
+
+#print deactivate_threads._match_1
+
+lemma vv {k} (ha : any_thread_active (deactivate_threads (bnot ∘ f) ac s)) (hi : exec_state k (deactivate_threads (bnot ∘ f) ac s) s t) (h : exec_state (loop f k) (deactivate_threads (bnot ∘ f) ac s) t u) :
+exec_state (loop f k) ac s u := begin
+    apply exec_state.loop_step,
+    repeat { assumption },
+    have hgest : deactivate_threads (bnot ∘ f) ac s ≥ deactivate_threads (bnot ∘ f) ac t := monotonic_exec hi,
+    generalize_hyp eq_ac : (deactivate_threads (bnot ∘ f) ac s) = dac at h hi, -- we need this, otherwise we have two disjoint ac
+    generalize_hyp eq_l : (loop f k) = l at h ⊢,
+    clear hi,
+    induction h;
+        cases eq_l;
+    subst eq_ac,
+    {
+        apply exec_state.loop_stop,
+        rw ac_deac_ge hgest at h_a,
+        exact h_a,
+    }, {
+        clear t u,
+        rename h_s t,
+        rename h_t t₂,
+        rename h_u u,
+        rename h_ih_a_1 ih,
+        rename h_a_1 htt₂,
+        clear h_ih_a,
+        rw ac_deac_ge hgest at htt₂,
+        have hgett₂ : deactivate_threads (bnot ∘ f) ac t ≥ deactivate_threads (bnot ∘ f) ac t₂ := monotonic_exec htt₂,
+        have hgest₂ : deactivate_threads (bnot ∘ f) ac s ≥ deactivate_threads (bnot ∘ f) ac t₂ := ac_trans hgest hgett₂,
+        specialize ih hgest₂ rfl rfl,
+        apply exec_state.loop_step,
+        swap 3,
+        apply ih,
+        rw ac_deac_ge hgest at h_a,
+        exact h_a,
+        exact htt₂,
+    }
+end
 
 example (k : kernel σ τ) (ac : vector bool n) (s s' : state n σ τ) : exec_state k ac s s' ↔ parlang.exec_state k ac s s' := begin
     split,
@@ -165,8 +371,8 @@ example (k : kernel σ τ) (ac : vector bool n) (s s' : state n σ τ) : exec_st
         }, {
             apply parlang.exec_state.loop_step,
             repeat { assumption },
-            have : monotone_loop h_f h_k h_s h_ac := by apply ac_ge_two,
-            
+            have : monotone_loop parlang.exec_state h_f h_k h_s h_ac := by apply ac_ge_two,
+            admit,
         },
     }, {
         intro h,
@@ -192,8 +398,9 @@ example (k : kernel σ τ) (ac : vector bool n) (s s' : state n σ τ) : exec_st
         }, {
             apply exec_state.loop_stop,
             assumption,
-        }, {
-            apply exec_state.loop_step,
+        }, 
+        case parlang.exec_state.loop_step : a b c ac f k' ha hel hek ih₁ ih₂ {
+            apply vv,
             repeat { assumption },
         },
     }
